src/Translation.v
@@ -50,15 +50,10 @@ Section translate_pattern.
     end.
 End translate_pattern.
 
-Ltac normilize_bool :=
-  repeat match goal with
-  | [ H : negb _ = true |- _ ] => rewrite negb_true_iff in H
-  | [ H : negb _ <> true |- _ ] => rewrite negb_true_iff in H
-  | [ H : _ = false |- _ ] => rewrite <- not_true_iff_false in H
-  | [ H : _ <> false |- _ ] => rewrite -> not_false_iff_true in H
-  | [ H : (In_decb _ _) = true |- _ ] => rewrite -> In_decb_true_iff in H
-  | [ H : (In_decb _ _) <> true |- _ ] => rewrite -> In_decb_true_iff in H
-  end.
+Ltac desf_translate_pvertex_pedge :=
+  unfold translate_pvertex, translate_pedge in *;
+  desf; simpls;
+  normalize_bool.
 
 Theorem translate_pattern__type_of pi n (Hwf : Pattern.wf pi) :
   (In n (Pattern.dom_edges pi) <-> type_of (translate_pattern pi) n = Some Value.GEdgeT) /\
@@ -66,18 +61,14 @@ Theorem translate_pattern__type_of pi n (Hwf : Pattern.wf pi) :
 Proof.
   all: induction pi; simpls.
   all: unfold Pattern.wf in *.
-  all: unfold translate_pvertex.
-  all: unfold translate_pedge.
 
   { do 2 split; ins; desf; simpls.
-    all: autounfold with unfold_pat in *.
-    all: desf; simpls.
-    all: eauto with pattern_wf_db.
-    all: unfold complement, equiv in *; contradiction. }
+    all: desf_translate_pvertex_pedge.
+    all: desf_unfold_pat.
+    all: Pattern.solve_wf_contra. }
 
   split.
-  all: desf; simpls.
-  all: normilize_bool.
+  all: desf_translate_pvertex_pedge.
   all: split; ins; desf.
 
   all: try now apply update_eq.
@@ -86,11 +77,9 @@ Proof.
   all: try rewrite update_neq.
   all: try (apply IHpi; [ split | ]; now eauto with pattern_wf_db).
 
-  all: try now (intros ?; exfalso; subst; eauto with pattern_wf_db).
-  all: try now (intros ?; exfalso; subst; simple eapply NoDup_cons_l; eassumption).
+  all: try now (intros ?; subst; Pattern.solve_wf_contra).
 
-  all: autounfold with unfold_pat in *.
-  all: desf; simpls.
+  all: desf_unfold_pat.
   all: try now (left; eauto with pattern_wf_db).
   all: right; apply IHpi; [ split | ]; now eauto with pattern_wf_db.
 Qed.
@@ -103,17 +92,23 @@ Corollary translate_pattern__type_of_GEdgeT pi n (Hwf : Pattern.wf pi) :
   (In n (Pattern.dom_edges pi) <-> type_of (translate_pattern pi) n = Some Value.GEdgeT).
 Proof. edestruct translate_pattern__type_of; eassumption. Qed.
 
+Theorem translate_pattern__type_of__types pi n :
+  type_of (translate_pattern pi) n = Some Value.GVertexT \/
+  type_of (translate_pattern pi) n = Some Value.GEdgeT \/
+  type_of (translate_pattern pi) n = None.
+Proof.
+  edestruct type_of_types as [H | [H | H]]; eauto.
+Qed.
+
 Corollary translate_pattern__type_of_None pi n (Hwf : Pattern.wf pi)
   (HIn_vertices : ~ In n (Pattern.dom_vertices pi))
   (HIn_edges    : ~ In n (Pattern.dom_edges pi)) :
     type_of (translate_pattern pi) n = None.
 Proof.
-  edestruct type_of_types as [H | [H | H]].
-  - eapply translate_pattern__type_of_GVertexT in H; try eassumption.
-    apply HIn_vertices in H. contradiction.
-  - eapply translate_pattern__type_of_GEdgeT in H; try eassumption.
-    apply HIn_edges in H. contradiction.
-  - assumption.
+  edestruct translate_pattern__type_of__types as [H | [H | H]]; eauto.
+  1: eapply translate_pattern__type_of_GVertexT in H; try eassumption.
+  2: eapply translate_pattern__type_of_GEdgeT in H; try eassumption.
+  all: congruence.
 Qed.
 
 Corollary translate_pattern__type_of_None_iff pi n (Hwf : Pattern.wf pi) :
@@ -136,7 +131,7 @@ Proof.
   2: assert (Pattern.wf pi) by (eapply Pattern.hop_wf; eassumption).
   all: unfold translate_pvertex, translate_pedge.
   all: desf; simpls; splits; auto.
-  all: normilize_bool.
+  all: normalize_bool.
   all: try apply translate_pattern__type_of_GVertexT; try assumption.
   all: try apply translate_pattern__type_of_None; try assumption.
   all: eauto with pattern_wf_db.
@@ -146,24 +141,417 @@ Proof.
   all: unfold complement, equiv in *.
   all: try contradiction.
   all: try apply translate_pattern__type_of_GVertexT; try assumption.
-  all: try (exfalso; simple eapply Pattern.wf__pe_neq_pv; eassumption).
-  all: try (exfalso; simple eapply Pattern.wf__pv_neq_pe; eassumption).
+  all: Pattern.solve_wf_contra.
 Qed.
 
-Module EvalQueryImpl (S : ExecutionPlan.Spec).
+Module EvalQueryImpl (S : ExecutionPlan.Spec) : EvalQuery.Spec.
   Module EvalPlanImpl := EvalPlan S.
   Import S.
   Import EvalPlanImpl.
 
-  Definition eval_pattern (graph : PropertyGraph.t) (pi : Pattern.t) : option BindingTable.t :=
+  Definition eval_match_clause (graph : PropertyGraph.t) (pi : Pattern.t) : option BindingTable.t :=
     let plan := translate_pattern pi in
       EvalPlanImpl.eval graph plan.
   
-  Theorem eval_pattern__wf graph pi
+  Theorem match_clause_wf graph pi
     (Hwf_g : PropertyGraph.wf graph) (Hwf : Pattern.wf pi) :
-      exists table', eval_pattern graph pi = Some table'.
+      exists table', eval_match_clause graph pi = Some table'.
   Proof.
     eapply eval_wf; eauto.
     now apply translate_pattern_wf.
+  Qed.
+
+  Theorem match_clause_type_of graph pi table'
+    (Hres : eval_match_clause graph pi = Some table') :
+    BindingTable.of_type table' (type_of (translate_pattern pi)).
+  Proof.
+    eapply eval_type_of; eassumption.
+  Qed.
+
+  Ltac desf_match_result Hres :=
+    unfold eval_match_clause in Hres; simpls;
+    desf_translate_pvertex_pedge;
+    unfold option_bind in *; desf.
+
+  Theorem match_clause_reduce graph pi pe pv table'
+    (Hres : eval_match_clause graph (Pattern.hop pi pe pv) = Some table') :
+      exists table, eval_match_clause graph pi = Some table.
+  Proof.
+    desf_match_result Hres.
+    all: eauto.
+  Qed.
+
+  Theorem match_clause_dom graph pi table' r'
+    (Hres : eval_match_clause graph pi = Some table')
+    (HIn : In r' table') :
+      Rcd.matches_pattern_dom r' pi.
+  Proof.
+    intros k.
+    unfold eval_match_clause in Hres.
+    rewrite Rcd.in_dom_iff, Pattern.In_dom.
+    erewrite match_clause_type_of; try eassumption.
+    clear Hres HIn.
+    split.
+
+    { intros [x Htype].
+      edestruct translate_pattern__type_of__types as [H | [H | H]].
+      all: erewrite H in Htype.
+      all: inv H.
+      all: induction pi; simpls.
+
+      all: desf_translate_pvertex_pedge.
+      all: desf_unfold_pat.
+
+      all: destruct IHpi; auto. }
+
+    { intros [HIn | HIn].
+      all: induction pi; simpls; desf.
+
+      all: desf_translate_pvertex_pedge.
+      all: try eauto using update_eq.
+      all: desf_unfold_pat.
+
+      all: try apply IHpi.
+      all: try now eexists.
+      all: congruence. }
+  Qed.
+
+  Lemma matches_pattern_dom_start r' pv v
+    (Hdom : Rcd.matches_pattern_dom r' (Pattern.start pv))
+    (Hval : r' (Pattern.vname pv) = Some (Value.GVertex v)) :
+      r' = (Pattern.vname pv |-> Value.GVertex v).
+  Proof.
+    extensionality k.
+    desf_unfold_pat.
+    unfold empty, t_empty.
+
+    unfold Rcd.matches_pattern_dom, Rcd.in_dom in *.
+    specialize Hdom with k; simpls.
+    destruct (r' k) eqn:Hval'; auto.
+
+    eassert (Hin : exists v, Some _ = Some v) by eauto.
+    rewrite Hdom in Hin.
+    desf.
+  Qed.
+
+  Lemma matches_pattern_dom_start' r' pv x
+    (Hval : r' = (Pattern.vname pv |-> x)) :
+      Rcd.matches_pattern_dom r' (Pattern.start pv).
+  Proof.
+    unfold Rcd.matches_pattern_dom in *; ins.
+    split; ins; desf.
+    all: unfold Rcd.in_dom in *.
+    all: desf.
+    all: try eexists.
+    all: desf_unfold_pat.
+    exfalso; eauto.
+  Qed.
+
+  Definition expansion_of_by_hop' graph r' r mode v_from e v_to pi pe pv :=
+    expansion_of' graph r' r mode v_from e v_to
+      (Pattern.vname (Pattern.last pi)) (Pattern.ename pe) (Pattern.vname pv) (Pattern.edir pe).
+
+  Definition expansion_of_by_hop graph r' r mode pi pe pv :=
+    expansion_of graph r' r mode
+      (Pattern.vname (Pattern.last pi)) (Pattern.ename pe) (Pattern.vname pv) (Pattern.edir pe).
+
+  Lemma matches_in_dom graph path pi r' n
+    (Hmatch : Path.matches graph r' path pi)
+    (HIn : In n (Pattern.dom pi)) :
+      exists x, r' n = Some x.
+  Proof.
+    induction Hmatch.
+    all: destruct Hpv; try destruct Hpe.
+    all: simpls; desf.
+    all: eauto.
+  Qed.
+
+  Lemma matches_in_dom_contra graph path pi r' n
+    (Hmatch : Path.matches graph r' path pi)
+    (Hval : r' n = None) :
+      ~ In n (Pattern.dom pi).
+  Proof.
+    intro contra.
+    eapply matches_in_dom in contra; eauto.
+    desf.
+  Qed.
+
+  Lemma matches_last graph path pi r'
+    (Hmatch : Path.matches graph r' path pi) :
+      r' (Pattern.vname (Pattern.last pi)) = Some (Value.GVertex (Path.last path)).
+  Proof.
+    destruct pi. 
+    all: inv Hmatch.
+    all: destruct Hpv; try destruct Hpe.
+    all: eauto.
+  Qed.
+
+  Lemma matches_exclude graph path pi r' n x
+    (Hmatch : Path.matches graph r' path pi)
+    (HIn : ~ In n (Pattern.dom pi)) :
+      Path.matches graph (n !-> x; r') path pi.
+  Proof.
+    induction Hmatch.
+    all: destruct Hpv; try destruct Hpe.
+    1: apply Path.matches_nil.
+    2: apply Path.matches_cons.
+    all: try apply IHHmatch.
+    all: try (intro; apply HIn; right; now right).
+    all: try apply Path.Build_matches_pvertex.
+    all: try apply Path.Build_matches_pedge.
+    all: auto.
+    all: desf_unfold_pat.
+    all: exfalso; auto.
+  Qed.
+
+  Lemma matches_pattern_dom_exclude_All pi pe pv r'
+    (Hwf : Pattern.wf (Pattern.hop pi pe pv))
+    (Hdom : Rcd.matches_pattern_dom r' (Pattern.hop pi pe pv))
+    (HIn : ~ In (Pattern.vname pv) (Pattern.dom_vertices pi)) :
+      Rcd.matches_pattern_dom (Pattern.ename pe !-> None; Pattern.vname pv !-> None; r') pi.
+  Proof.
+    unfold Rcd.matches_pattern_dom in *.
+    intros k. specialize Hdom with k.
+    split; intro H.
+    all: unfold Rcd.in_dom in *.
+    all: desf_unfold_pat.
+    { destruct Hdom as [? | [? | ?]]; eauto.
+      all: exfalso; eauto. }
+    all: rewrite Pattern.In_dom in *; desf.
+    all: try Pattern.solve_wf_contra.
+  Qed.
+
+  Lemma matches_pattern_dom_exclude_Into pi pe pv r'
+    (Hwf : Pattern.wf (Pattern.hop pi pe pv))
+    (Hdom : Rcd.matches_pattern_dom r' (Pattern.hop pi pe pv))
+    (HIn : In (Pattern.vname pv) (Pattern.dom_vertices pi)) :
+      Rcd.matches_pattern_dom (Pattern.ename pe !-> None; r') pi.
+  Proof.
+    unfold Rcd.matches_pattern_dom in *.
+    intros k. specialize Hdom with k.
+    split; intro H.
+    all: unfold Rcd.in_dom in *.
+    all: desf_unfold_pat.
+    { destruct Hdom as [? | [? | ?]]; subst; eauto.
+      all: now (rewrite Pattern.In_dom; eauto). }
+    all: rewrite Pattern.In_dom in *; desf.
+    all: try Pattern.solve_wf_contra.
+  Qed.
+
+  Lemma matches_hop_All graph path e v pi pe pv r'
+    (Hwf : Pattern.wf (Pattern.hop pi pe pv))
+    (Hdom : Rcd.matches_pattern_dom r' (Pattern.hop pi pe pv))
+    (Hmatch : Path.matches graph r' (Path.hop path e v) (Pattern.hop pi pe pv))
+    (HIn : ~ In (Pattern.vname pv) (Pattern.dom_vertices pi)) :
+      exists r, << Hexp : expansion_of_by_hop graph r' r All pi pe pv >> /\
+                << Hmatch' : Path.matches graph r path pi >> /\
+                << Hdom' : Rcd.matches_pattern_dom r pi >>.
+  Proof.
+    exists (Pattern.ename pe !-> None; Pattern.vname pv !-> None; r').
+    inv Hmatch.
+    destruct Hpe, Hpv.
+    eauto.
+    splits.
+    { unfold expansion_of_by_hop, expansion_of, expansion_of'.
+      do 3 eexists. splits; eauto.
+      
+      all: try extensionality k.
+      all: desf_unfold_pat.
+      all: try Pattern.solve_wf_contra.
+      { exfalso. apply HIn. rewrite e0. apply Pattern.last__dom_vertices. }
+      eauto using matches_last. }
+    { apply matches_exclude. apply matches_exclude.
+      { assumption. }
+      all: rewrite Pattern.In_dom.
+      all: intro; desf.
+      all: Pattern.solve_wf_contra. }
+    { apply matches_pattern_dom_exclude_All; eauto. }
+  Qed.
+
+  Lemma matches_hop_Into graph path e v pi pe pv r'
+    (Hwf : Pattern.wf (Pattern.hop pi pe pv))
+    (Hdom : Rcd.matches_pattern_dom r' (Pattern.hop pi pe pv))
+    (Hmatch : Path.matches graph r' (Path.hop path e v) (Pattern.hop pi pe pv))
+    (HIn : In (Pattern.vname pv) (Pattern.dom_vertices pi)) :
+      exists r, << Hexp : expansion_of_by_hop graph r' r Into pi pe pv >> /\
+                << Hmatch' : Path.matches graph r path pi >> /\
+                << Hdom' : Rcd.matches_pattern_dom r pi >>.
+  Proof.
+    exists (Pattern.ename pe !-> None; r').
+    inv Hmatch.
+    destruct Hpe, Hpv.
+    eauto.
+    splits.
+    { unfold expansion_of_by_hop, expansion_of, expansion_of'.
+      do 3 eexists. splits; eauto.
+      
+      all: try extensionality k.
+      all: desf_unfold_pat.
+      all: try Pattern.solve_wf_contra.
+      eauto using matches_last. }
+    { apply matches_exclude.
+      { assumption. }
+      all: rewrite Pattern.In_dom.
+      all: intro; desf.
+      all: Pattern.solve_wf_contra. }
+    { eapply matches_pattern_dom_exclude_Into; eauto. }
+  Qed.
+
+  Theorem match_clause_spec graph path pi table' r'
+    (Hres : eval_match_clause graph pi = Some table')
+    (Hwf : Pattern.wf pi)
+    (Hdom : Rcd.matches_pattern_dom r' pi)
+    (Hmatch : Path.matches graph r' path pi) :
+      In r' table'.
+  Proof.
+    generalize dependent Hdom.
+    generalize dependent Hres.
+    generalize dependent r'.
+    generalize dependent table'.
+    generalize dependent path.
+    induction pi; ins.
+    all: destruct path; inv Hmatch.
+    all: destruct Hpv.
+    all: try destruct Hpe.
+
+    { all: desf_match_result Hres.
+      1: eapply filter_vertices_by_label_spec; try eassumption.
+      all: auto.
+      all: assert (r' = (Pattern.vname pv |-> Value.GVertex v))
+            by (eauto using matches_pattern_dom_start); subst.
+      all: eauto using scan_vertices_spec. }
+
+    all: desf_match_result Hres.
+    all: repeat match goal with
+         | [H : filter_by_label Vertices _ _ _ _ = _ |- _ ] =>
+            eapply filter_vertices_by_label_spec; try eassumption; clear H
+         | [H : filter_by_label Edges _ _ _ _ = _ |- _ ] =>
+            eapply filter_edges_by_label_spec; try eassumption; clear H
+         end.
+    all: auto.
+    all: match goal with 
+         | [H : expand Into _ _ _ _ _ _ = _ |- _ ] =>
+            apply matches_hop_Into in Hmatch; eauto
+         | [H : expand All _ _ _ _ _ _ = _ |- _ ] =>
+            apply matches_hop_All in Hmatch; eauto
+         end.
+    all: desf.
+    all: match goal with
+         | [H : expand _ _ _ _ _ _ _ = _ |- _ ] =>
+            eapply expand_spec; eauto
+         end.
+    all: eapply IHpi.
+    all: eauto with pattern_wf_db.
+  Qed.
+
+  Lemma matches_pattern_dom_hop graph mode r r' pi pe pv
+    (* (Hwf : Pattern.wf pi) *)
+    (Hdom : Rcd.matches_pattern_dom r pi)
+    (Hexp : expansion_of_by_hop graph r' r mode pi pe pv) :
+      Rcd.matches_pattern_dom r' (Pattern.hop pi pe pv).
+  Proof.
+    unfold expansion_of_by_hop, expansion_of, expansion_of' in Hexp.
+    unfold Rcd.matches_pattern_dom, Rcd.in_dom in *.
+    ins; desf; desf.
+    all: split; ins; desf.
+    all: desf_unfold_pat.
+    all: try rewrite <- Hdom.
+    all: eauto.
+    all: try now (exfalso; eauto).
+    all: try now rewrite -> Hdom.
+  Qed.
+
+  Lemma matches_expansion_of graph mode r r' path v_from e v_to pi pe pv
+    (Hg_wf : PropertyGraph.wf graph)
+    (Hwf : Pattern.wf (Pattern.hop pi pe pv))
+    (Hdom : Path.matches graph r path pi)
+    (Hvlabel : forall l : label, Pattern.vlabel pv = Some l -> In l (vlabels graph v_to))
+    (Helabel : forall l : label, Pattern.elabel pe = Some l -> elabel graph e = l)
+    (Hexp : expansion_of_by_hop' graph r' r mode v_from e v_to pi pe pv) :
+      Path.matches graph r' (Path.hop path e v_to) (Pattern.hop pi pe pv).
+  Proof.
+    apply Path.matches_cons.
+    all: unfold expansion_of_by_hop', expansion_of', expansion_of in Hexp.
+    all: desf; desf.
+    all: try apply matches_exclude.
+    all: try apply matches_exclude.
+    all: eauto using matches_in_dom_contra.
+    all: try apply Path.Build_matches_pedge.
+    all: try apply Path.Build_matches_pvertex.
+    all: auto.
+
+    all: assert (Path.last path = v_from)
+          by (erewrite matches_last in Hval_from; eauto;
+            injection Hval_from; trivial).
+    all: subst; auto.
+
+    all: try now rewrite update_eq.
+    all: try rewrite update_neq.
+    all: try now rewrite update_eq.
+    all: try assumption.
+    all: try Pattern.solve_wf_contra.
+
+    all: unfold Path.matches_direction in Hdir.
+    all: desf; desf.
+    all: edestruct ends_In; eauto.
+  Qed.
+
+  Theorem match_clause_spec' graph pi table' r'
+    (Hres : eval_match_clause graph pi = Some table')
+    (Hg_wf : PropertyGraph.wf graph)
+    (Hwf : Pattern.wf pi)
+    (HIn : In r' table') :
+      exists path, Path.matches graph r' path pi /\
+        Rcd.matches_pattern_dom r' pi.
+  Proof.
+    generalize dependent Hres.
+    generalize dependent r'.
+    generalize dependent table'.
+    induction pi; ins.
+    all: desf_match_result Hres.
+    all: repeat match goal with
+         | [H : filter_by_label Vertices _ _ _ _ = _ |- _ ] =>
+            eapply filter_vertices_by_label_spec' in H; try eassumption; desf
+         | [H : filter_by_label Edges _ _ _ _ = _ |- _ ] =>
+            eapply filter_edges_by_label_spec' in H; try eassumption; desf
+         end.
+    all: try match goal with
+          | [H : scan_vertices _ _ = _ |- _ ] =>
+             eapply scan_vertices_spec' in H; try eassumption; desf
+          end.
+    all: repeat match goal with
+         | [H : expand _ _ _ _ _ _ _ = _ |- _ ] =>
+            eapply expand_spec' in H; try eassumption; desf
+         end.
+    all: try edestruct IHpi as [path [? ?]];
+            eauto with pattern_wf_db.
+    all: unfold expansion_of_by_hop, expansion_of in *; desf.
+    1-2: eexists (Path.start _); splits.
+    5-12: eexists (Path.hop path _ _); splits.
+
+    all: try eapply matches_expansion_of; eauto.
+    all: try eapply matches_pattern_dom_hop.
+    all: try unfold expansion_of_by_hop, expansion_of.
+    all: eauto using matches_pattern_dom_start'.
+
+    all: try eapply Path.matches_nil, Path.Build_matches_pvertex; eauto.
+    all: try rewrite update_eq.
+    all: auto.
+
+    all: ins.
+    all: try unfold expansion_of' in *; desf.
+    all: repeat match goal with
+          | [H1 : ?x = ?y, H2 : ?x = ?z |- _ ] =>
+              rewrite H1 in H2; inj_subst; subst
+          | [H : (?x |-> ?y) ?x = Some ?z |- _ ] =>
+              rewrite update_eq in H; injection H as H; subst
+          | [H : (?x |-> ?y; _) ?x = Some ?z |- _ ] =>
+              rewrite update_eq in H; injection H as H; subst
+          | [H : (Pattern.ename _ |-> _; _) _ = Some (Value.GVertex _) |- _ ] =>
+              rewrite -> update_neq in H; [ | Pattern.solve_wf_contra ]
+          | [H : (Pattern.vname _ |-> _; _) _ = Some (Value.GEdge _) |- _ ] =>
+              rewrite -> update_neq in H; [ | Pattern.solve_wf_contra ]
+          end.
+    all: auto.
   Qed.
 End EvalQueryImpl.
